HoareSim wand rule

proofmode/HSim.v
@@ -1215,7 +1215,55 @@ Section SIM.
     { gstep. econs 16; eauto. gbase. eapply rclo9_clo_base. left. econs; eauto. }
   Qed.
 
-(* TODO: frame, wand *)
+  Variant hwandC (r: forall R_src R_tgt
+                            (Q: Any.t -> Any.t -> R_src -> R_tgt -> iProp)
+                            (ctx: Σ),
+                     option Ord.t -> bool -> bool -> Any.t * itree hEs R_src -> Any.t * itree Es R_tgt -> Prop)
+          {R_src R_tgt}
+          (Q: Any.t -> Any.t -> R_src -> R_tgt -> iProp)
+          (ctx: Σ)
+    : option Ord.t -> bool -> bool -> Any.t * itree hEs R_src -> Any.t * itree Es R_tgt -> Prop :=
+    | hwandC_intro
+        f_src f_tgt fuel Q0
+        st_src st_tgt
+        (SIM: r _ _ Q0 ctx fuel f_src f_tgt st_src st_tgt)
+        (WAND: forall st_src st_tgt ret_src ret_tgt,
+            (bi_entails (Q0 st_src st_tgt ret_src ret_tgt) (#=> Q st_src st_tgt ret_src ret_tgt)))
+      :
+      hwandC r Q ctx fuel f_src f_tgt st_src st_tgt
+  .
+
+  Lemma hwandC_mon:
+    monotone9 hwandC.
+  Proof. ii. inv IN; econs; et. Qed.
+  Hint Resolve hwandC_mon: paco.
+
+  Lemma hwandC_spec: hwandC <10= gupaco9 (_hsim) (cpn9 _hsim).
+  Proof.
+    eapply wrespect9_uclo; eauto with paco.
+    econs; eauto with paco. i. inv PR. eapply GF in SIM.
+    induction SIM using _hsim_ind2; i; clarify; ired_both.
+    { econs 1; eauto. eapply current_iProp_upd.
+      eapply current_iProp_entail; eauto.
+    }
+    { econs 2; eauto. i. eapply rclo9_clo_base. econs; eauto. }
+    { econs 3; eauto. }
+    { econs 4; eauto. des. esplits; eauto. i. hexploit SIM; eauto. i. eapply rclo9_clo_base. econs; eauto. }
+    { econs 5; eauto. i. eapply rclo9_clo_base. econs; eauto. }
+    { econs 6; eauto. }
+    { econs 7; eauto. }
+    { econs 8; eauto. des. esplits; eauto. }
+    { econs 9; eauto. i. hexploit SIM; eauto. i. des. esplits; eauto. }
+    { econs 10; eauto. i. hexploit SIM; eauto. i. des. esplits; eauto. }
+    { econs 11; eauto. des. esplits; eauto. }
+    { econs 12; eauto. }
+    { econs 13; eauto. }
+    { econs 14; eauto. }
+    { econs 15; eauto. }
+    { econs 16; eauto. eapply rclo9_clo_base. econs; eauto. }
+  Qed.
+
+(* TODO: frame *)
 
 
 End SIM.
